examples/log/DiskLogSystem.dfy
@@ -1,0 +1,45 @@
+include "DiskLog.dfy"
+include "Disk.dfy"
+
+module DiskLogSystem {
+  import M = DiskLog
+  import D = Disk
+
+  datatype Constants = Constants(disk: D.Constants, machine: M.Constants)
+  datatype Variables = Variables(disk: D.Variables<M.LBAType.LBA, M.Sector>, machine: M.Variables)
+
+  predicate Init(k: Constants, s: Variables)
+  {
+    && M.Mkfs(k.machine, k.disk, s.disk)
+    && M.Init(k.machine, s.machine)
+  }
+
+  datatype Step =
+    | MachineStep(diskOp: M.DiskOp)
+    | CrashStep
+
+  predicate Machine(k: Constants, s: Variables, s': Variables, diskOp: M.DiskOp)
+  {
+    && M.Next(k.machine, s.machine, s'.machine, diskOp)
+    && D.Next(k.disk, s.disk, s'.disk, diskOp)
+  }
+
+  predicate Crash(k: Constants, s: Variables, s': Variables)
+  {
+    && M.Init(k.machine, s'.machine)
+    && s'.disk == s.disk
+  }
+
+  predicate NextStep(k: Constants, s: Variables, s': Variables, step: Step)
+  {
+    match step {
+      case MachineStep(diskOp) => Machine(k, s, s', diskOp)
+      case CrashStep => Crash(k, s, s')
+    }
+  }
+
+  predicate Next(k: Constants, s: Variables, s': Variables) {
+    exists step :: NextStep(k, s, s', step)
+  }
+  
+}
